theories/simplang/class_instances.v
@@ -242,7 +242,7 @@ Section irreducible.
     destruct (heap σ !! l) as [ [[ |  ] ] | ] eqn:Heq; decide_goal.
   Qed.
   Global Instance irreducible_freeN σ v_l v_n P :
-    IrredUnless (∃ l n, v_l = LitV $ LitLoc l ∧ v_n = LitV $ LitInt n ∧ (0 < n)%Z ∧
+    IrredUnless (∃ l n, v_l = LitV $ LitLoc l ∧ v_n = LitV $ LitInt n ∧ (0 < n)%Z ∧ block_is_dyn l.(loc_block) ∧
                        (∀ m : Z, is_Some (heap σ !! (l +ₗ m)) ↔ (0 ≤ m < n)%Z))
       P (FreeN (Val v_n) (Val v_l)) σ.
   Proof.
@@ -253,6 +253,7 @@ Section irreducible.
     apply (exists_dec_unique n); [ naive_solver|].
     apply and_dec; [decide_goal|].
     apply and_dec; [decide_goal|].
+    apply and_dec; [apply _|].
     apply and_dec; [apply _|].
     apply forall_equiv_dec.
     - destruct (decide (map_Forall (λ l' _,
@@ -312,10 +313,10 @@ Section irreducible.
       intros (l & ? & ? & ?); eauto).
   Qed.
   Global Instance irreducible_freeN_weak σ v_l v_n P :
-    IrredUnless (∃ l n, v_l = LitV $ LitLoc l ∧ v_n = LitV $ LitInt n ∧ (0 < n)%Z) P (FreeN (Val v_n) (Val v_l)) σ | 10.
+    IrredUnless (∃ l n, v_l = LitV $ LitLoc l ∧ v_n = LitV $ LitInt n ∧ (0 < n)%Z ∧ block_is_dyn l.(loc_block)) P (FreeN (Val v_n) (Val v_l)) σ | 10.
   Proof.
     eapply irred_unless_weaken; last apply irreducible_freeN.
-    intros (l & ? & ? & ? &? &?); eauto 8.
+    intros (l & ? & ? & ? &? &? &?); eauto 8.
   Qed.
 End irreducible.
 
